Update lec5

src/sys_verif/coq/verifying_functional.v
@@ -161,39 +161,136 @@ writing `db_rep : database -> M` what should `M` be?
 |*)
 
 
+(*| ### Example 2: map with deletions |*)
+
+(* This Module just groups the definitions so we can use short names inside. *)
+Module deleteMap.
+
+(* the values in the map don't matter so we pick something arbitrary *)
+Notation V := nat.
+
+(* This type of inductive is common enough that we could replace this
+boilerplate with the [Record] feature. We use an inductive only to avoid
+introducing new syntax. *)
+Inductive map :=
+  | mkMap (elements: gmap Z V) (deletions: gset Z).
+Definition elements (m: map) : gmap Z V :=
+  match m with
+  | mkMap elements _ => elements
+  end.
+Definition deletions (m: map) : gset Z :=
+  match m with
+  | mkMap _ deletions => deletions
+  end.
+
+(* The underscore will distinguish these names from the std++ map definitions,
+which we'll use as the spec. *)
+Definition empty_ : map := mkMap ∅ ∅.
+Definition insert_ (k: Z) (v: V) (m: map) : map :=
+  mkMap (insert k v (elements m)) (deletions m ∖ {[k]}).
+Definition remove_ (k: Z) (m: map) : map :=
+  mkMap (elements m) (deletions m ∪ {[k]}).
+Definition lookup_ (k: Z) (m: map) : option V :=
+  if decide (k ∈ deletions m) then None
+  else (elements m) !! k.
+
+Definition rep (m: map) : gmap Z V :=
+  (* to remove all the deletions, we filter to the (k, v) pairs where k is _not_
+  deleted *)
+  filter (λ '(k, v), k ∉ deletions m) (elements m).
+
+Lemma empty_spec : rep empty_ = ∅.
+Proof.
+  rewrite /rep /=.
+  reflexivity.
+Qed.
+Lemma insert_spec k v m : rep (insert_ k v m) = insert k v (rep m).
+Proof.
+  rewrite /rep /=.
+  apply map_eq. intros k'.
+  destruct (decide (k' = k)).
+  - subst. rewrite lookup_insert.
+    apply map_lookup_filter_Some.
+    rewrite lookup_insert.
+    split.
+    + auto.
+    + set_solver.
+  - rewrite lookup_insert_ne //.
+    (* figured this out by trial and error (after finding the two relevant
+    lemmas) *)
+    rewrite map_filter_insert_True.
+    { set_solver. }
+    rewrite lookup_insert_ne //.
+    admit.
+Admitted.
+Lemma remove_spec k m : rep (remove_ k m) = delete k (rep m).
+Proof.
+  rewrite /rep /=.
+  apply map_eq. intros k'.
+  destruct (decide (k' = k)).
+  - subst. rewrite lookup_delete.
+    apply map_lookup_filter_None.
+    set_solver.
+  - rewrite lookup_delete_ne //.
+    admit.
+Admitted.
+Lemma lookup_spec k m : lookup_ k m = (rep m) !! k.
+Proof.
+  rewrite /rep /=.
+  rewrite /lookup_.
+  destruct (decide _).
+  - rewrite map_lookup_filter_None_2 //.
+    set_solver.
+  - destruct (elements m !! k) eqn:H.
+    + symmetry.
+      apply map_lookup_filter_Some_2; auto.
+    + rewrite map_lookup_filter_None_2 //.
+      set_solver.
+Qed.
+End deleteMap.
+
 (*| ## Model-based specification |*)
 
 (*| This is the generic form of the spec we saw above for big integers.
 
-Starting point: have some data structure or other object of type T (the _code_
-or _concrete_ representation). It consists of:
+Starting point: want to verify an Abstract Data Type (ADT, not to be confused
+with _algebraic data type_). An ADT consists of:
 
+- A type `T` (the _code_ or _concrete_ representation) of the data type.
 - Initialization (constructors or "introduction"). For some `A: Type`, `init: A → T`
 - Methods: for some `A: Type`, `op: T → A → T`
 - Getters ("eliminators"): of the form `f: T → A` for some `A: Type`.
 
-1. The first step is to pick a type `S` that will be the _abstract_ representation
-(or _model_) of the data of type `T`. (Note: in general, `S` will not efficient in the programming
-language, or might not even be representable).
-2. Invent an _abstraction function_ `rep : T → S` giving what abstract value the
-code is representing.
-3. Prove specs for each function:
-    - Write `init_spec : A → S`. Prove `∀ (v: A), rep (init v) = init_spec v`.
-    - Write `op_spec : S → A → S`. Prove `∀ (x: T) (v: A), rep (op x v) = op_spec (rep x) v`.
-    - Write `f_spec: S → A`. Prove `∀ (x: T), f x = f_spec (rep x)`.
+A specification for an ADT is constructed similarly:
+
+1. Come up with a model for the code.
+   * Pick a type `S` that will be the _abstract_ representation (or _model_) of
+     the data of type `T`. (Note: in general, `S` will not efficient in the
+     programming language, or might not even be representable).
+   * Write a version of each code function in terms of the abstract type `S`
+     rather than `T`: `init_spec : A → S`, `op_spec : S → A → S`, and `f_spec :
+     S → A`.
+2. To relate the code to the model, invent an _abstraction function_ `rep : T →
+   S` giving what abstract value the code is representing.
+3. Prove the following obligations that relate the code to the model via the abstraction function:
+    - For `init_spec : A → S`, prove `∀ (v: A), rep (init v) = init_spec v`.
+    - For `op_spec : S → A → S`, prove `∀ (x: T) (v: A), rep (op x v) = op_spec (rep x) v`.
+    - For `f_spec: S → A`, prove `∀ (x: T), f x = f_spec (rep x)`.
 
 ::: important Model-based specifications
 
 Make sure you can follow what the specifications above are actually saying. It
 might not all make sense at this point but after seeing examples come back to
 this description. We'll revisit it a couple more times as the basis for
-specifying imperative and concurrent programs.
+specifying imperative and concurrent programs, where the code will be more
+sophisticated and we'll need to do more work to relate the code to the model,
+which will remain mathematical functions.
 
 :::
 
 Why prove the above? These obligations show that any sequence of operations can
-be understood in terms of `_spec` variants, even though we run the concrete
-versions:
+be understood in terms of model (the `_spec` variants of each function), even
+though we run the concrete versions. For example this code:
 
 ```
 let x := init c1;
@@ -204,7 +301,8 @@ r
 ```
 
 This whole process produces `get_result (do_op2 (do_op1 (init c1)))` when the
-code is run.  But at an abstract level we could just as well have written:
+code is run. We can instead view this as the following sequence, using the
+model:
 
 ```
 let x' := init_spec c1;
@@ -215,7 +313,20 @@ r'
 ```
 
 **Claim:** `r' = r` if the data structure satisfies the specs described above.
-(Check that you believe this!)
+
+We can use the proofs above to prove this claim that `r' = r`, using simple
+equational reasoning; at each step we are applying one obligation from the
+above.
+
+```
+  r
+= get_result      (do_op2      (do_op1      (init c1)))
+= get_result_spec (abs (do_op2 (do_op1      (init c1))))
+= get_result_spec (do_op2_spec (abs (do_op1 (init c1))))
+= get_result_spec (do_op2_spec (do_op1_spec (abs (init c1))))
+= get_result_spec (do_op2_spec (do_op1_spec (init_spec c1)))
+= r'
+```
 
 :::: important Client-centric reasoning
 
@@ -231,14 +342,17 @@ Sometimes described as a **commutative diagram** (though this term has a very
 specific meaning in category theory which is likely the more common usage of
 "commutative diagram").
 
-Notice that the claim does not depend on `rep`; it is a detail of the proof that
-explains _why_ the code is correct, but is not necessary to understand _what the
-code does_. On the other hand if you were verifying the code you would certainly
-care about what `rep` is, and if you were writing it you also might want to
-think about how each code state maps to the desired abstraction.
+Notice that the client reasoning does not depend on `rep`; it is a detail of the
+proof that explains _why_ the code is correct, but is not necessary to
+understand _what the code does_. On the other hand if you were verifying the
+code you would certainly care about what `rep` is since it directly shows up in
+all of the proof obligations, and if you were implementing this library you also
+might want to have a model in mind and think about how each code state maps to
+it.
 
-Also notice that `S` and all the spec variants were invented as part of the
-spec. You can even imagine two different specs for the same code.
+Also notice that the model - `S` and all the spec variants - were invented as
+part of the spec, but aren't inheret to the code. You can even imagine proving
+the same code relates to two different models.
 
 |*)
 
@@ -268,6 +382,58 @@ Make an attempt to write the proof obligations for a model-based specification
 that incorporates an invariant over the data, adapting the strategy above. Think
 about what would make your strategy _sound_ in justifying the reasoning above
 that converted the code functions to spec functions.
+
+|*)
+
+(*| ## Lecture 5: model-based specifications, continued {#lec5} |*)
+(*| ### Learning outcomes
+1. State a model-based specification for an ADT that uses an invariant
+2. Compare equational specifications to model-based specifications
+|*)
+
+(*| 
+### Review: invariant-based specification
+
+Adding invariants to the model-based specification above:
+
+1. Same as above: create a model with `S`, `init_spec`, `op_spec`, and `f_spec.
+2. Pick `rep : T → S` but also pick `inv : T → Prop`.
+3. Prove obligations for each function:
+    - For `init_spec : A → S`, prove `∀ (v: A), rep (init v) = init_spec v` (as above) AND `∀ v, inv (init v)`.
+    - For `op_spec : S → A → S`, prove `∀ (x: T) (v: A), inv x → rep (op x v) = op_spec (rep x) v ∧ inv (op x v)`.
+    - For `f_spec: S → A`, prove `∀ (x: T), inv x → f x = f_spec (rep x)`.
+
+Observe how these obligations prove that any value `y: T` produced from using
+this interface will satisfy `inv y`.
+
+Second, notice that we get to assume `inv x` as a premise, which is what makes
+this more powerful, but we're also on the hook to prove `inv x` is actually
+initially true and maintained (to justify assuming it). Invariants are tricky to
+come up with for this reason. However, without the ability to use an invariant,
+these obligations require reasoning about any value of type `T`, which may just
+be impossible
+
+Finally, a small observation: the strategy is _strictly_ more powerful than
+without invariants; we can always pick `inv x = True` and then it's the same as
+if we didn't have an invariant at all.
+
+### Exercise: re-do client-centric reasoning
+
+- $T : \mathrm{Type}$
+- $i : T$
+- $op_1 : T \to T$ and $op_2 : T \to T$
+- $f : T \to A$
+
+And the spec:
+
+- $S : \mathrm{Type}$, $rep : T \to S$, and $inv : T \to \mathrm{Prop}$
+- $i' : S$
+- $op_1' : S \to S$ and $op_2' : S \to S$
+- $f' : S \to A$
+
+Prove that $f' (op_2' (op_1'(i'))) = f (op_2 (op_1 (i)))$ using the theorems
+above. (Note we typically write $f(x)$ for blackboard/on-paper reasoning on the
+blackboard/paper while the same function application is written `f x` in Coq).
 
 |*)
 
@@ -350,8 +516,11 @@ Proof.
   - simpl.
     set_solver.
   - simpl.
+    intros Hinv.
     destruct (decide (x < el)).
-    + simpl. set_solver.
+    + simpl.
+      (* fairly powerful automation is used here *)
+      set_solver.
     + destruct (decide (el < x)).
       * simpl. set_solver.
       * simpl.
@@ -363,17 +532,16 @@ Lemma find_spec t x :
   st_inv t →
   st_find t x = bool_decide (x ∈ st_rep t).
 Proof.
+  (* this follows directly from the definition of [bool_decide] *)
   replace (bool_decide (x ∈ st_rep t)) with
     (if decide (x ∈ st_rep t) then true else false)
     by reflexivity.
-  intros Hinv.
   induction t.
-  - simpl.
+  - simpl. intros Hinv.
     set_solver.
-  - simpl.
+  - simpl. intros Hinv.
     destruct (decide (x < el)).
-    + simpl.
-      simpl in Hinv. destruct Hinv as (Hlt & Hgt & Hinvt1 & Hinvt2).
+    + destruct Hinv as (Hlt & Hgt & Hinvt1 & Hinvt2).
       rewrite IHt1.
       { auto. }
       destruct (decide (x ∈ st_rep t1)).
@@ -389,11 +557,11 @@ Proof.
           apply Hgt in Hel.
           lia. }
         set_solver.
-    + simpl in Hinv. destruct Hinv as (Hlt & Hgt & Hinvt1 & Hinvt2).
+    + destruct Hinv as (Hlt & Hgt & Hinvt1 & Hinvt2).
       destruct (decide (el < x)).
       * rewrite -> IHt2 by auto.
-        (* NOTE: you could do the rest of this proof with the more basic
-        techniques, as above. This is a more automated version. *)
+        (* NOTE: you could do the rest of this proof with more basic techniques,
+        as above. This is a more automated version. *)
         clear IHt1. (* needed to make [destruct] pick the right instance *)
         destruct (decide _); destruct (decide _); set_solver by lia.
       * assert (x = el) by lia.
@@ -402,9 +570,113 @@ Proof.
 Qed.
 
 (*| 
+## Invariant vs non-invariant spec styles
+
+A specification has two sides: the perspective of the implementor proving it, in
+which case it's an _obligation_, and the perspective of the client using it, in
+which case it's an _assumption_. In general the implementor wants
+(a) true obligations (they can't prove something false) and (b) simple
+obligations (if possible, they want to prove something easier than something
+harder). The client wants (a) strong enough to reason about their own code, and
+(b) easy-to-use specifications are preferred to strong but hard-to-understand
+ones.
+
+There is a tension here that the abstract spec is trying to balance.
+
+When we add invariants to the model-based specification, the benefit is that it
+allows us to prove _more ADTs correct_, and in fact many ADTs are only correct
+because they maintain some internal invariant (the implementor now has a hope of
+proving their code against this specification, like in the search tree example).
+There's no cost to the client, either, since essentially the same client
+reasoning works regardless of what the invariant is.
+
+|*)
+
+(*| 
 ## Beyond the above specification
 
-### Non-determinism: abstraction relations
+### Equational specifications
+
+A completely different style than the above is to give _equational_ or
+_algebraic_ specifications. An example where this makes a lot of sense is
+`encode`/`decode` functions. The main property we generally want of such
+functions (as a _client_ or user of such code) is a "round trip" theorem that
+says `∀ x, decode (encode x) = x`. There isn't even an obvious "model" to
+describe encoding or decoding.
+
+The danger of equational or algebraic specifications is that it's harder to
+think about whether the specification is good enough for client reasoning - in
+general need to give specs for any combination of functions. It has the
+advantage of not requiring an abstraction.
+
+|*)
+
+(*| ### Equational spec for maps |*)
+
+(*| Here is an ADT implementing maps that we'll prove equational properties
+for, rather than relating it to `gmap`. Think of this as what you would do if
+_implementing_ `gmap`, except we'll discuss later how `gmap` has a more
+complicated implementation to make it easier to use. |*)
+
+Definition list_map (K: Type) {H: EqDecision K} (V: Type) :=
+  list (K * V).
+
+(*| Sections are a way of writing a bunch of definitions that need to take the
+same types, like the `K`, `H: EqDecision K`, and `V` parameters for `list_map`.
+|*)
+Section list_map.
+
+(* To understand the code below, all you need to know is that `K` and `V` are
+defined as arbitrary types by this `Context` command. When the section is
+closed, all of these will become arguments to the definitions in the section for
+any users of this code (and there are no users yet for this little example). *)
+Context {K: Type} {H: EqDecision K} {V: Type}.
+
+Definition empty_list_map : list_map K V := [].
+
+Fixpoint find (x: K) (m: list_map K V) : option V :=
+  match m with
+  | [] => None
+  | (x', v) :: m' => if decide (x = x') then Some v else find x m'
+  end.
+
+Definition update (x : K) (v: V) (m: list_map K V) : list_map K V :=
+  (x, v) :: m.
+
+(*| What equations might we want? One idea is that we should prove something
+about any combinations of `find` and `update` we can think of (that type check).
+|*)
+
+Lemma find_empty_list_map x :
+  find x empty_list_map = None.
+Proof. reflexivity. Qed.
+
+Lemma find_update_eq (m: list_map K V) x v :
+  find x (update x v m) = Some v.
+Proof.
+  rewrite /update. simpl.
+  rewrite -> decide_True by auto.
+  reflexivity.
+Qed.
+
+Lemma find_update_neq (m: list_map K V) x y o :
+  x ≠ y → find x (update y o m) = find x m.
+Proof.
+  intros Hne.
+  rewrite /update. simpl.
+  rewrite -> decide_False by auto.
+  reflexivity.
+Qed.
+
+(*| At this point, have we proven all the equations that might be needed? I
+believe so, but it's hard to be sure, and the situation is worse when we have
+many operations that can interact with each other. |*)
+
+End list_map.
+
+(*| ## Extension 2: abstraction relations
+
+There's one more extension beyond invariants that allows us to
 
 There's one more extension that is natural to add at some point:
 non-determinism. Instead of `abs : T → S` (a function), we can instead have
@@ -426,21 +698,68 @@ provable with an abstraction relation.
 Another direction you might want to think about how we could add non-determinism
 to both the code operations and the spec operations, although this will take us
 away from functional programs so we won't consider it just yet.
-
-### Equational specifications
-
-A completely different style than the above is to give _equational_ or
-_algebraic_ specifications. An example where this makes a lot of sense is
-`encode`/`decode` functions. The main property we generally want of such
-functions (as a _client_ or user of such code) is a "round trip" theorem that
-says `∀ x, decode (encode x) = x`. There isn't even an obvious "model" to
-describe encoding or decoding.
-
-The danger of equational or algebraic specifications is that it's harder (and
-not systematic) to think about whether the specification is good enough for
-client reasoning. However, in the encode/decode example it's at some level it's
-necessary for the clients purposes to prove the round-trip property mentioned
-above.
-
 |*)
+
+Module stat_db.
+  Unset Printing Records.
+
+  (*| We use `Record` here to create an inductive type, which defines a
+  constructor `mkDb` as well as _projection functions_ `db_sum` and `db_num`.
+
+  Records in Coq have some special associated syntax for constructors and
+  projections, but we're not using it (and disable printing with that syntax as
+  well). |*)
+  Record database :=
+    mkDb { db_sum : Z; db_num : Z; }.
+
+  Definition empty_db : database := mkDb 0 0.
+  Definition insert_el (x: Z) (db: database) :=
+    mkDb (db_sum db + x) (db_num db + 1).
+  (* We're going to ignore division by zero. Coq makes [x / 0 = 0] which is how
+  this function will also work (this makes good mathematical sense which I'm
+  happy to explain, but it doesn't affect this example). *)
+  Definition mean (db: database) : Z :=
+    db_sum db / db_num db.
+
+  Definition failed_rep_function (db: database) : list Z := []. (* where do we get this from? *)
+
+  Definition listZ_sum (s: list Z) :=
+    foldl (λ s x, s + x) 0 s.
+
+  Definition absr (db: database) (s: list Z) :=
+    db_sum db = listZ_sum s ∧
+    db_num db = Z.of_nat (length s).
+
+  Lemma insert_el_spec x db s :
+    absr db s →
+    absr (insert_el x db) (s ++ [x]).
+  Proof.
+    rewrite /absr /=.
+    destruct db as [sum num]; simpl.
+    intros [Heq1 Heq2]. rewrite Heq1. rewrite Heq2.
+    split.
+    - rewrite /listZ_sum.
+      rewrite foldl_app /=.
+      reflexivity.
+    - rewrite length_app /=.
+      lia.
+  Qed.
+
+  (* this theorem follows pretty much immediately from the definitions of [absr]
+  and [mean]; the work is in maintaining [absr], not in this theorem *)
+  Lemma mean_spec db s :
+    absr db s →
+    mean db = listZ_sum s / (Z.of_nat (length s)).
+  Proof.
+    rewrite /absr /=.
+    destruct db as [sum num]; simpl.
+    (* instead of using [rewrite] we use [subst] because if `x = ...` and `x` is
+    a variable, we can replace it everywhere and then the equation is
+    redundant. *)
+    intros [? ?]; subst.
+    rewrite /mean /=.
+    reflexivity.
+  Qed.
+
+End stat_db.
 
